src/lib/data/Kuiper.Array3.fst
@@ -11,11 +11,16 @@ module Tac = FStar.Tactics.V2
 let desc (d0 d1 d2 : nat) : idesc 3 =
   d0 @| d1 @| d2 @| INil
 
-let adapt_idx (#d0 #d1 #d2 : nat) (idx : abs (desc d0 d1 d2)) : natlt d0 & natlt d1 & natlt d2 =
+let adapt_idx (#d0 #d1 #d2 : nat) (idx : abs (desc d0 d1 d2)) : ait d0 d1 d2 =
   match idx with
   | (i, (j, (k, ()))) -> (i, j, k)
 
-let adapt_idx_back (#d0 #d1 #d2 : nat) (idx : natlt d0 & natlt d1 & natlt d2) : abs (desc d0 d1 d2) =
+let adapt_idx_back (#d0 #d1 #d2 : nat) (idx : ait d0 d1 d2) : abs (desc d0 d1 d2) =
+  match idx with
+  | (i, j, k) -> (i, (j, (k, ())))
+
+inline_for_extraction noextract
+let adapt_cit_back (d0 d1 d2 : erased nat) (idx : raw_cit{cit_fits d0 d1 d2 idx}) : conc (desc d0 d1 d2) =
   match idx with
   | (i, j, k) -> (i, (j, (k, ())))
 
@@ -27,7 +32,7 @@ let tr_layout (#d0 #d1 #d2 : nat) (l : layout d0 d1 d2) : tlayout (desc d0 d1 d2
 #pop-options
 
 #push-options "--ifuel 3" // sigh
-let abs_bij (#d0 #d1 #d2 : nat) : (abs (desc d0 d1 d2) =~ (natlt d0 & natlt d1 & natlt d2)) =
+let abs_bij (#d0 #d1 #d2 : nat) : (abs (desc d0 d1 d2) =~ (ait d0 d1 d2)) =
   {
     ff = (fun (i, (j, (k, ()))) -> (i, j, k));
     gg = (fun (i, j, k) -> (i, (j, (k, ()))));
@@ -169,9 +174,7 @@ fn read
   (#d0 #d1 #d2 : erased nat)
   (#l : layout d0 d1 d2) {| clayout l |}
   (a : t et l)
-  (i : szlt d0)
-  (j : szlt d1)
-  (k : szlt d2)
+  (idx : raw_cit{cit_fits d0 d1 d2 idx})
   (#f : perm)
   (#s : erased (EMatrix3.t et d0 d1 d2))
   preserves
@@ -179,10 +182,10 @@ fn read
   returns
     v : et
   ensures
-    pure (v == EMatrix3.macc s i j k)
+    pure (v == EMatrix3.macc s (pi_3_0 idx) (pi_3_1 idx) (pi_3_2 idx))
 {
   unfold pts_to a #f s;
-  let v = T.tensor_read a (i, (j, (k, ())));
+  let v = T.tensor_read a (adapt_cit_back d0 d1 d2 idx);
   fold pts_to a #f s;
   v
 }
@@ -194,19 +197,19 @@ fn write
   (#d0 #d1 #d2 : erased nat)
   (#l : layout d0 d1 d2) {| clayout l |}
   (a : t et l)
-  (i : szlt d0)
-  (j : szlt d1)
-  (k : szlt d2)
+  (idx : raw_cit{cit_fits d0 d1 d2 idx})
   (v : et)
   (#s : erased (EMatrix3.t et d0 d1 d2))
-  requires a |-> s
-  ensures  a |-> EMatrix3.mupd s i j k v
+  requires
+    a |-> s
+  ensures
+    a |-> EMatrix3.mupd s (pi_3_0 idx) (pi_3_1 idx) (pi_3_2 idx) v
 {
   unfold pts_to a s;
-  T.tensor_write a (i, (j, (k, ()))) v;
+  T.tensor_write a (adapt_cit_back d0 d1 d2 idx) v;
   with cs'. assert T.tensor_pts_to a cs';
-  assert pure (Chest.equal cs' (tr_val (EMatrix3.mupd s i j k v)));
-  fold pts_to a (EMatrix3.mupd s i j k v);
+  assert pure (Chest.equal cs' (tr_val (EMatrix3.mupd s (pi_3_0 idx) (pi_3_1 idx) (pi_3_2 idx) v)));
+  fold pts_to a (EMatrix3.mupd s (pi_3_0 idx) (pi_3_1 idx) (pi_3_2 idx) v);
   ()
 }
 #pop-options
@@ -215,14 +218,14 @@ let pts_to_cell
   (#et : Type) (#d0 #d1 #d2 : nat) (#l : layout d0 d1 d2)
   ([@@@mkey] a : t et l)
   (#[Tac.exact (`1.0R)] f : perm)
-  ([@@@mkey] ijk : natlt d0 & natlt d1 & natlt d2)
+  ([@@@mkey] ijk : ait d0 d1 d2)
   (v : et)
   : slprop
   = T.tensor_pts_to_cell a #f (adapt_idx_back ijk) v
 
 let pts_to_cell_eq
   (#et : Type) (#d0 #d1 #d2 : nat) (#l : layout d0 d1 d2)
-  (a : t et l) (ijk : natlt d0 & natlt d1 & natlt d2) (f : perm) (v : et)
+  (a : t et l) (ijk : ait d0 d1 d2) (f : perm) (v : et)
   : Lemma (pts_to_cell a #f ijk v
            ==
            gpu_pts_to_cell (core a) #f (l.imap.f ijk) v)
@@ -236,13 +239,13 @@ fn explode
   (#s : EMatrix3.t et d0 d1 d2)
   requires a |-> Frac f s
   ensures
-    forall+ (ijk : natlt d0 & natlt d1 & natlt d2).
+    forall+ (ijk : ait d0 d1 d2).
       Cell a ijk |-> Frac f (EMatrix3.macc s (pi_3_0 ijk) (pi_3_1 ijk) (pi_3_2 ijk))
 {
   unfold pts_to a #f s;
   T.tensor_explode a;
   forevery_iso abs_bij _;
-  forevery_ext _ (fun (ijk : natlt d0 & natlt d1 & natlt d2) -> Cell a ijk |-> Frac f (EMatrix3.macc s (pi_3_0 ijk) (pi_3_1 ijk) (pi_3_2 ijk)));
+  forevery_ext _ (fun (ijk : ait d0 d1 d2) -> Cell a ijk |-> Frac f (EMatrix3.macc s (pi_3_0 ijk) (pi_3_1 ijk) (pi_3_2 ijk)));
   ()
 }
 
@@ -255,7 +258,7 @@ fn implode
   requires
     pure (SZ.fits (layout_size l))
   requires
-    forall+ (ijk : natlt d0 & natlt d1 & natlt d2).
+    forall+ (ijk : ait d0 d1 d2).
       Cell a ijk |-> Frac f (EMatrix3.macc s (pi_3_0 ijk) (pi_3_1 ijk) (pi_3_2 ijk))
   ensures
     a |-> Frac f s
